Done with a major refactor

tests/lean/run/cbv1.lean
@@ -1,9 +1,10 @@
 set_option trace.Meta.Tactic.cbv true
 
-def myId (n : Nat): Nat := match n with
-  | 0 => 0
-  | n + 1 => myId n + 1
-theorem lambdaTest : (myId 1).succ = 2 := by
+def myId (l : List α) : Nat := match l with
+  | [] => 0
+  | (_ :: _) => 1
+
+theorem lambdaTest : (myId ([] : List Nat) ).succ = 1 := by
   conv =>
     lhs
     cbv
@@ -12,8 +13,6 @@ def issue : (fun (α) (l : List α) => l) Nat ([] : List Nat) = [] := by
   conv =>
     lhs
     cbv
-
-#print issue
 
 theorem dependentMatchIssue : [2,3,4].length = 3 := by
   conv =>
@@ -30,26 +29,12 @@ def myFun (n : Nat) : Nat :=
   termination_by id n
 
 -- /- We need to be able to normalize this to a `OfNat.ofNat` -/
-theorem myFunCbv : have x := 17; myFun x = 17 := by
-  grind [myFun]
-
--- /--
-
--- error: Tactic `simp` failed with a nested error:
--- maximum recursion depth has been reached
--- use `set_option maxRecDepth <num>` to increase limit
--- use `set_option diagnostics true` to get diagnostic information
--- -/
--- #guard_msgs in
--- theorem myFunSimp : myFun 170 = 170 := by
---   simp [myFun]
-
-
--- /- Triggers an error due to having free variables under the lambda -/
-
-
-theorem free_variable_issue : (fun y => (fun x : Nat => if true then y else true)) false = (fun _ => false) := by
+theorem myFunCbv : myFun 170 = 170 := by
   conv =>
     lhs
     cbv
-  rfl
+
+theorem free_variable_issue : (fun y => (fun x : Nat => if true then y else true)) false = (fun x => if true = true then false else true) := by
+  conv =>
+    lhs
+    cbv
